compiler/backend/semantics/closSemScript.sml
@@ -159,7 +159,19 @@ val do_install_def = Define `
             | _ => (Rerr(Rabort Rtype_error),s))
        | _ => (Rerr(Rabort Rtype_error),s))`;
 
-val do_app_def = Define `
+Definition make_const_def:
+  make_const (ConstInt i) = Number i ∧
+  make_const (ConstStr s) = ByteVector (MAP (n2w o ORD) s) ∧
+  make_const (ConstWord64 w) = Word64 w ∧
+  make_const (ConstCons t cs) = Block t (MAP make_const cs)
+Termination
+  WF_REL_TAC ‘measure const_size’
+  \\ Induct_on ‘cs’ \\ rw []
+  \\ fs [const_size_def] \\ res_tac
+  \\ pop_assum (qspec_then ‘t’ assume_tac) \\ fs []
+End
+
+Definition do_app_def:
   do_app (op:closLang$op) (vs:closSem$v list) ^s =
     case (op,vs) of
     | (Global n,[]:closSem$v list) =>
@@ -174,6 +186,7 @@ val do_app_def = Define `
     | (AllocGlobal,[]) =>
         Rval (Unit, s with globals := s.globals ++ [NONE])
     | (Const i,[]) => Rval (Number i, s)
+    | (Constant c,[]) => Rval (make_const c, s)
     | (Cons tag,xs) => Rval (Block tag xs, s)
     | (ConsExtend tag, Block _ xs'::Number lower::Number len::Number tot::xs) =>
         if lower < 0 ∨ len < 0 ∨ &LENGTH xs' < lower + len ∨
@@ -384,7 +397,8 @@ val do_app_def = Define `
     | (LessConstSmall n,[Number i]) =>
         (if 0 <= i /\ i <= 1000000 /\ n < 1000000 then Rval (Boolv (i < &n),s) else Error)
     | (ConfigGC,[Number _; Number _]) => (Rval (Unit, s))
-    | _ => Error`;
+    | _ => Error
+End
 
 val dec_clock_def = Define `
 dec_clock n ^s = s with clock := s.clock - n`;
